Introduce MonadSkipLawsE and GeneralizeIterLawsE. Use MonadLawsE instead of MonadLaws. Use Interaction Trees in the implementation of [div].

theories/div.v
@@ -1,175 +1,85 @@
 From stdpp Require Import base.
+From ITree Require Import ITree Eq Exception ITreeMonad.
 Require Import monads.
 
 (* ------------------------------------------------------------------------ *)
 
-(* A divergence monad. *)
+(* A divergence and failure monad. *)
 
-(* This type is co-inductive and offers a [Skip] constructor, as usual in
-   a divergence monad. It also offers a hard failure constructor [Fail]. *)
+(* This type is co-inductive and offers a [skip] operation for silent steps,
+   as usual in a divergence monad. It also offers a hard failure operation,
+   modeled as an exception that carries a unit argument. *)
 
-(* This type COULD be viewed as an instance of the type [itree] offered by
-   the Interaction Trees library. *)
-
-CoInductive div A :=
-  | Ret (a : A)
-  | Fail
-  | Skip (m : div A).
-
-Arguments Ret {A} a.
-Arguments Fail {A}.
-Arguments Skip {A} m.
+Definition div A :=
+  itree (exceptE unit) A.
 
 (* ------------------------------------------------------------------------ *)
 
-(* Monadic combinators. *)
-
-(* [subst f m] is [bind m f]. Defining [subst] first allows us to point out
-   to Coq that the argument [f] is invariant (i.e., it does not change as
-   the cofixpoint is unfolded). This in turn allows Coq to accept more
-   co-inductive definitions that involve [bind]; the definition of [iter]
-   is an example. *)
-
-Section Subst.
-
-  Context {A B : Type}.
-  Variable (f : A → div B).
-
-  CoFixpoint subst (m : div A) : div B :=
-    match m with
-    | Ret a =>
-        f a
-    | Fail =>
-        Fail
-    | Skip m =>
-        Skip (subst m)
-    end.
-
-End Subst.
-
-(* [bind] is [subst] with its argument reversed. *)
-
-Definition bind {A B} (m : div A) (f : A → div B) : div B :=
-  subst f m.
+(* Because [itree] is a monad, [div] is a monad. *)
 
 Global Instance monad_div : Monad div :=
-  { ret := @Ret; bind := @bind }.
+  Monad_itree.
+
+Arguments monad_div /.
+
+(* We use [eutt], also known as [≈], as the natural notion of equality
+   between computations. That said, some of the statements below would
+   hold also with a stronger equality; e.g. [MonadSkipLawE] would hold
+   with strong bisimulation [≅]. *)
+
+Global Instance eq1_div : Eq1 div :=
+  Eq1_ITree.
+
+Arguments eq1_div /.
+
+(* ------------------------------------------------------------------------ *)
+
+(* [skip] is a silent step. *)
+
+Definition div_skip {A} (m : div A) :=
+  Tau m.
+
+Arguments div_skip {A} m /.
 
 Global Instance monadskip_div : MonadSkip div :=
-  { skip := @Skip }.
+  { skip := @div_skip }.
+
+Arguments monadskip_div /.
+
+Local Ltac msimpl :=
+  unfold Proper, eq1; simpl;
+  unfold Eq1_ITree; simpl.
 
 Global Instance monadskiplaws_div :
-  MonadSkipLaws _ _.
+  MonadSkipLawsE monad_div monadskip_div.
 Proof.
-  constructor; simpl. intros.
-  unfold bind, skip, monadskip_div.
-Admitted.
-
-(* ------------------------------------------------------------------------ *)
-
-(* Equality of monadic computations. *)
-
-CoInductive eq {A} : div A → div A → Prop :=
-| EqRet a :
-    eq (Ret a) (Ret a)
-| EqFail :
-    eq Fail Fail
-| EqSkip m1 m2 :
-    eq m1 m2 →
-    eq (Skip m1) (Skip m2)
-.
-
-Local Hint Constructors eq : eq.
-
-Local Infix "~" := eq (at level 70, no associativity).
-
-(* Equality is reflexive, symmetric, and transitive. *)
-
-Lemma eq_reflexive {A} :
-  ∀ (m : div A),
-  m ~ m.
-Proof.
-  cofix CH. destruct m; constructor; eauto.
+  constructor.
+  (* Proper_skip *)
+  { msimpl. intros A m1 m2. unfold skip; simpl. intros.
+    (* We exploit the fact that equality ignores [Tau] steps. That said,
+       this congruence property would be true even if we used a stronger
+       equality that does not ignore silent steps. *)
+    do 2 rewrite tau_eutt. assumption. }
+  (* bind_skip *)
+  { msimpl. intros. unfold skip; simpl.
+    (* The lemma [bind_tau] is a strong bisimulation statement. A fortiori,
+       a weak bisimulation statement holds as well. *)
+    rewrite bind_tau. reflexivity. }
 Qed.
 
-Lemma eq_symmetric {A} :
-  ∀ m1 m2 : div A,
-  m1 ~ m2 →
-  m2 ~ m1.
-Proof.
-  cofix CH. inversion 1; subst; constructor; eauto.
-Qed.
-
-Lemma eq_transitive {A} :
-  ∀ m1 m2 m3 : div A,
-  m1 ~ m2 → m2 ~ m3 → m1 ~ m3.
-Proof.
-Admitted.
-
-Local Hint Resolve eq_reflexive : eq.
-
 (* ------------------------------------------------------------------------ *)
 
-(* The monadic laws. *)
-
-Lemma monad_law_left_unit {A B} (a : A) (f : A → div B) :
-  bind (Ret a) f ~ f a.
-Proof.
-  replace (bind (Ret a) f) with (f a). 2: admit.
-  apply eq_reflexive.
-Admitted.
-
-Lemma monad_law_right_unit {A} :
-  ∀ (m : div A),
-  bind m Ret ~ m.
-Proof.
-  cofix CH. destruct m.
-  { apply monad_law_left_unit. }
-  { replace (bind Fail Ret) with (Fail : div A). 2: admit.
-    apply eq_reflexive. }
-  { replace (bind (Skip m) Ret) with (Skip (bind m Ret)). 2: admit.
-    constructor. eauto. }
-Admitted.
-
-Lemma monad_law_associativity :
-  ∀ {A B C} (m : div A) (g : A → div B) (h : B → div C),
-  bind (bind m g) h ~
-  bind m (λ a, bind (g a) h).
-Proof.
-Abort.
-
-(* ------------------------------------------------------------------------ *)
-
-(* We cannot define a general fixed point combinator. This definition
-   is not accepted by Coq, as the function [ff] could deconstruct its
-   argument:
-
-   CoFixpoint mfix {T U} (ff : (T → div U) → (T → div U)) (t : T) : div U :=
-     ff (λ t, Skip (mfix ff t)) t.
-
- *)
-
-(* ------------------------------------------------------------------------ *)
-
-(* We can however define an iteration combinator [iter]. *)
-
-CoFixpoint div_iter {R I} (body : I → div (I + R)) (i : I) : div R :=
-  (* Evaluate [body] out of the state [i]. *)
-  bind (body i) (λ (signal : I + R),
-    match signal with
-    | inl i =>
-        (* If the body yields a new state [i], continue. *)
-        Skip (div_iter body i)
-    | inr r =>
-        (* If the body yields a result [r], return this result. *)
-        Ret r
-    end).
+(* An iteration combinator [iter] is available. *)
 
 Global Instance monaditer_div : MonadIter div :=
-  { iter := @div_iter }.
+  MonadIter_itree.
+
+Arguments monaditer_div /.
 
 Global Instance monaditerlaws_div :
-  MonadIterLaws _ _ _.
+  MonadIterLawsE _ _ _.
 Proof.
-  constructor. simpl.
-Admitted.
+  constructor. msimpl. unfold skip, iter; simpl. intros.
+  (* The lemma [Eqit.unfold_iter] is a strong bisimulation statement. *)
+  rewrite Eqit.unfold_iter. reflexivity.
+Qed.
