theories/handle.v
@@ -1,5 +1,4 @@
-Require Import lang eval monads.
-Require free.
+Require Import lang monads free eval.
 
 (* This file defines an interpretation (a transformation) of the [free]
    monad into a monad equipped with [mzero] and [mfix] combinators. *)
@@ -7,14 +6,17 @@ Require free.
 Section Handle.
 
 Context {target : Type → Type}.
+Context {EQ1 : Eq1 target}.
+Local Open Scope monad_scope.
 Context {M : Monad target}.
-Context {ML : MonadLaws M}.
+Context {EQ1Equivalence : Eq1Equivalence target}.
+Context {ML : MonadLawsE target}.
 Context {MZ : MonadZero target}.
 Context {MZL : MonadZeroLaws M MZ}.
 Context {MS : MonadSkip target}.
-Context {MSL : MonadSkipLaws M MS}.
+Context {MSL : MonadSkipLawsE M MS}.
 Context {MI : MonadIter target}.
-Context {MIL : MonadIterLaws M MI MS}.
+Context {MIL : MonadIterLawsE M MI MS}.
 
 Section A.
 
@@ -24,18 +26,18 @@ Context {A : Type}.
 
 (* An interpretation of our free monad into the target monad. *)
 
-Definition handle_body (m : free.mon A) : target (free.mon A + A) :=
+Definition handle_body (m : free A) : target (free A + A) :=
   match m with
-  | free.Ret a =>
+  | Ret a =>
       (* Termination is mapped to termination. *)
       ret (inr a)
-  | free.Fail =>
+  | Fail =>
       (* Hard failure is mapped to hard failure. *)
       mzero
-  | free.Next =>
+  | Next =>
       (* Soft failure is not expected to happen. *)
       mzero
-  | free.Stop (free.REval η e) k =>
+  | Stop (REval η e) k =>
       (* A [Stop] effect is mapped to an invocation of [eval]. The call
          [eval η e] is composed with the continuation [k]. This computation
          is then transported from the free monad into the target monad via
@@ -43,12 +45,12 @@ Definition handle_body (m : free.mon A) : target (free.mon A + A) :=
       ret (inl (bind (eval η e) k))
   end.
 
-Definition handle : free.mon A → target A :=
+Definition handle : free A → target A :=
   iter handle_body.
 
-Lemma handle_fixed_point (m : free.mon A) :
-  handle m =
-    bind (handle_body m) (fun (signal : free.mon A + A) =>
+Lemma handle_fixed_point (m : free A) :
+  handle m ≈
+    bind (handle_body m) (fun (signal : free A + A) =>
       match signal with
       | inl m =>
           skip (handle m)
@@ -62,15 +64,15 @@ Qed.
 (* Paraphrase lemmas. *)
 
 Lemma handle_ret (a : A) :
-  handle (free.Ret a) = ret a.
+  handle (Ret a) ≈ ret a.
 Proof.
   rewrite handle_fixed_point. unfold handle_body.
-  rewrite bind_of_return by typeclasses eauto.
+  rewrite bind_ret_l.
   reflexivity.
 Qed.
 
 Lemma handle_fail :
-  handle (free.Fail : free.mon A) = mzero.
+  handle Fail ≈ mzero.
 Proof.
   rewrite handle_fixed_point. unfold handle_body.
   rewrite bind_zero by typeclasses eauto.
@@ -78,19 +80,19 @@ Proof.
 Qed.
 
 Lemma handle_next :
-  handle (free.Next : free.mon A) = mzero.
+  handle Next ≈ mzero.
 Proof.
   rewrite handle_fixed_point. unfold handle_body.
   rewrite bind_zero by typeclasses eauto.
   reflexivity.
 Qed.
 
-Lemma handle_stop η e (k : val → free.mon A) :
-  handle (free.Stop (free.REval η e) k) =
+Lemma handle_stop η e (k : val → free A) :
+  handle (free.Stop (free.REval η e) k) ≈
   skip (handle (bind (eval η e) k)).
 Proof.
-  rewrite (handle_fixed_point (free.Stop _ _)). unfold handle_body.
-  rewrite bind_of_return by typeclasses eauto.
+  rewrite (handle_fixed_point (Stop _ _)). unfold handle_body.
+  rewrite bind_ret_l.
   reflexivity.
 Qed.
 
@@ -110,31 +112,32 @@ Definition run η e : target val :=
 
 (* In other words, [handle] is a monad morphism. *)
 
-Lemma compatibility {A B} (m : free.mon A) :
-  ∀ (f : A → free.mon B),
-  bind (handle m) (λ v, handle (f v)) =
+Lemma compatibility {A B} (m : free A) :
+  ∀ (f : A → free B),
+  bind (handle m) (λ v, handle (f v)) ≈
   handle (bind m f).
 Proof.
   induction m as [ | | | [ η e] k IH ]; intros.
   { rewrite handle_ret.
-    do 2 rewrite bind_of_return by typeclasses eauto.
+    do 2 rewrite bind_ret_l.
     reflexivity. }
-  { rewrite free.free_bind_fail.
+  { rewrite bind_fail.
     do 2 rewrite handle_fail.
     rewrite bind_zero by typeclasses eauto.
     reflexivity. }
-  { rewrite free.free_bind_next.
+  { rewrite bind_next.
     do 2 rewrite handle_next.
     rewrite bind_zero by typeclasses eauto.
     reflexivity. }
-  { rewrite free.free_bind_stop.
+  { rewrite bind_stop.
     do 2 rewrite handle_stop.
-    rewrite bind_skip by typeclasses eauto. f_equal.
+    rewrite bind_skip by typeclasses eauto.
+    eapply Proper_skip; try solve [ typeclasses eauto ].
     (* TODO We are in trouble: we are trying to establish something
        that looks like the initial goal,
        where [m] has been instantiated with [eval η e]. *)
     generalize (eval η e); intros m. clear η e.
-    rewrite <- bind_associativity by typeclasses eauto.
+    rewrite <- bind_bind.
     generalize (bind m k). clear m k IH. intros m.
     (* This is exactly the original goal... *)
     (* We may need some form of co-induction:
