theories/wp.v
@@ -1,4 +1,4 @@
-Require Import lang free eval spec handle.
+Require Import monads lang free eval spec handle.
 
 (* Instantiate the generic [handle] with the [spec] monad. *)
 
@@ -31,11 +31,25 @@ Definition example :=
 
 Eval cbv in eval EnvNil example.
 
+Lemma handle_fixed_point_paraphrase {A} (m : free A) :
+  handle m =
+    bind (handle_body m) (fun (signal : free A + A) =>
+      match signal with
+      | inl m =>
+          skip (handle m)
+      | inr r =>
+          ret r
+      end).
+Proof.
+  eapply @handle_fixed_point.
+  typeclasses eauto.
+Qed.
+
 (* An example of reasoning about straight-line code. *)
 
 Goal wp EnvNil example (λ v, v = VData "A" (VTuple VNil)).
 Proof.
-  cbv. rewrite handle_fixed_point. cbv. reflexivity.
+  cbv. rewrite handle_fixed_point_paraphrase. cbv. reflexivity.
 Qed.
 
 (* let x = (z1, z2) in let (x1, x2) = x in x1 *)
@@ -50,5 +64,5 @@ Goal
   let env := EnvCons "z1" v1 (EnvCons "z2" v2 EnvNil) in
   wp env example2 (λ v, v = v1).
 Proof.
-  intros. cbv. rewrite handle_fixed_point. cbv. reflexivity.
+  intros. cbv. rewrite handle_fixed_point_paraphrase. cbv. reflexivity.
 Qed.
